Carefully revert "Implement dynamic, GooseLang-based types and memory operations (#224)"
This reverts commit a4bf5daec1b5220730183ff8f8165674501e915d.

new/golang/defn/array.v
@@ -1,35 +1,28 @@
 From New Require Import notation.
 From New.golang.defn Require Import typing list.
 
-(** Fixed-size arrays.
-
-NOTE: this library is incomplete, even the signatures here could be wrong.
-*)
-
 Module array.
 Section defn.
   Context `{ffi_syntax}.
 
-  Definition elem_ref : val :=
-    λ: "et" "a" "i", Panic "todo".
+  Definition elem_ref (t : go_type) : val.
+  Admitted.
 
-  Definition elem_get : val :=
-    λ: "et" "a" "i", Panic "todo".
+  Definition elem_get (t : go_type) : val.
+  Admitted.
 
-  (* t here is the array type, not the element type *)
-  Definition len : val :=
-    λ: "t", Panic "todo".
+  Definition len (t : go_type) : val.
+  Admitted.
 
-  (* t here is the array type, not the element type *)
-  Definition cap : val :=
-    λ: "t", len "t".
+  Definition cap (t : go_type) : val.
+  Admitted.
 
-  Definition slice : val :=
-    λ: "t" "a", Panic "todo".
+  Definition slice : val.
+  Admitted.
 
   (* takes a list as input, and makes an array value *)
   Definition literal : val :=
     rec: "literal" "len" "elems" :=
-      list.Match "elems" (λ: <>, #()) (λ: "hd" "tl", ("hd", "literal" "tl")).
+      list.Match (λ: <>, #()) (λ: "hd" "tl", ("hd", "literal" "tl")).
 End defn.
 End array.
