new/golang/theory/slice.v
@@ -3,8 +3,7 @@ From iris.algebra Require Import dfrac.
 From Perennial.iris_lib Require Import dfractional.
 From Perennial.goose_lang Require Import ipersist.
 From New.golang.defn Require Export slice.
-From New.golang.theory Require Import list assume exception loop typing primitive auto.
-From New.golang.theory Require Import mem.
+From New.golang.theory Require Export list mem assume exception loop typing primitive auto.
 From Perennial Require Import base.
 
 Set Default Proof Using "Type".
@@ -377,7 +376,7 @@ Context `{!IntoValTyped V t}.
 Lemma wp_slice_make3 stk E (len cap : w64) :
   uint.nat len ≤ uint.nat cap →
   {{{ True }}}
-    slice.make3 #t #len #cap @ stk; E
+    slice.make3 t #len #cap @ stk; E
   {{{ sl, RET #sl;
       sl ↦* (replicate (uint.nat len) (default_val V)) ∗
       own_slice_cap V sl (DfracOwn 1) ∗
@@ -439,6 +438,7 @@ Proof.
     rewrite /own_slice_cap_def /=.
     iSplitR; first iPureIntro.
     { word. }
+    rewrite default_val_eq_zero_val.
     erewrite has_go_type_len.
     2:{ apply zero_val_has_go_type. }
     iExists (replicate (uint.nat cap - uint.nat len)%nat (default_val V)).
@@ -460,7 +460,7 @@ Qed.
 
 Lemma wp_slice_make2 stk E (len : u64) :
   {{{ True }}}
-    slice.make2 #t #len @ stk; E
+    slice.make2 t #len @ stk; E
   {{{ sl, RET #sl;
       sl ↦* (replicate (uint.nat len) (default_val V)) ∗
       own_slice_cap V sl (DfracOwn 1)
@@ -500,19 +500,18 @@ Proof.
 Qed.
 
 Global Instance pure_elem_ref s (i : w64) :
-  PureWp (uint.Z i < uint.Z s.(slice.len_f)) (slice.elem_ref #t #s #i)
+  PureWp (uint.Z i < uint.Z s.(slice.len_f)) (slice.elem_ref t #s #i)
     #(slice.elem_ref_f s t i).
 Proof.
   iIntros (?????) "HΦ".
   wp_call_lc "?".
   rewrite bool_decide_true; last done.
-  wp_pures. wp_apply wp_array_loc_add. iIntros "_".
-  by iApply "HΦ".
+  wp_pures. by iApply "HΦ".
 Qed.
 
 Global Instance pure_slice_slice s (n m : w64) :
   PureWp (uint.Z n ≤ uint.Z m ≤ uint.Z (slice.cap_f s) ∧
-          uint.Z (slice.len_f s) ≤ uint.Z (slice.cap_f s)) (slice.slice #t #s #n #m)
+          uint.Z (slice.len_f s) ≤ uint.Z (slice.cap_f s)) (slice.slice t #s #n #m)
     #(slice.slice_f s t n m).
 Proof.
   iIntros (?????) "HΦ".
@@ -524,10 +523,9 @@ Proof.
   rewrite bool_decide_true; last word.
   wp_pures.
   iDestruct ("HΦ" with "[$]") as "HΦ".
-  wp_apply wp_array_loc_add. iIntros "_".
-  wp_pures.
   iExactEq "HΦ".
   repeat f_equal.
+  rewrite /slice.slice_f.
   rewrite !to_val_unseal /=.
   rewrite !to_val_unseal /=.
   reflexivity.
@@ -535,7 +533,7 @@ Qed.
 
 Global Instance pure_full_slice s (n m c : w64) :
   PureWp (uint.Z n ≤ uint.Z m ≤ uint.Z c ∧
-          uint.Z c ≤ uint.Z (slice.cap_f s)) (slice.full_slice #t #s #n #m #c)
+          uint.Z c ≤ uint.Z (slice.cap_f s)) (slice.full_slice t #s #n #m #c)
     #(slice.full_slice_f s t n m c).
 Proof.
   iIntros (?????) "HΦ".
@@ -549,7 +547,6 @@ Proof.
   rewrite bool_decide_true; last word.
   wp_pures.
   iDestruct ("HΦ" with "[$]") as "HΦ".
-  wp_apply wp_array_loc_add. iIntros "_". wp_pures.
   iExactEq "HΦ".
   repeat f_equal.
   rewrite /slice.full_slice_f.
@@ -566,7 +563,7 @@ this lemma would be pretty much unnecessary.
 Lemma wp_slice_slice_pure s (n m: w64) :
   {{{ ⌜uint.Z n ≤ uint.Z m ≤ uint.Z s.(slice.cap_f) ∧
         uint.Z s.(slice.len_f) ≤ uint.Z s.(slice.cap_f)⌝ }}}
-    slice.slice #t #s #n #m
+    slice.slice t #s #n #m
   {{{ RET #(slice.slice_f s t n m); True }}}.
 Proof.
   wp_start as "%".
@@ -757,7 +754,7 @@ instead
 *)
 Lemma wp_slice_slice s dq (vs: list V) (n m : w64) :
   {{{ s ↦*{dq} vs ∗ ⌜uint.Z n ≤ uint.Z m ≤ uint.Z s.(slice.len_f)⌝ }}}
-    slice.slice #t #s #n #m
+    slice.slice t #s #n #m
   {{{ RET #(slice.slice_f s t n m);
       (* before the sliced part *)
       (slice.slice_f s t (W64 0) n) ↦*{dq} (take (uint.nat n) vs) ∗
@@ -783,7 +780,7 @@ instead
 Lemma wp_slice_slice_with_cap s (vs: list V) (n m : w64) :
   {{{ s ↦* vs ∗ own_slice_cap V s (DfracOwn 1) ∗
             ⌜uint.Z n ≤ uint.Z m ≤ uint.Z s.(slice.len_f)⌝ }}}
-    slice.slice #t #s #n #m
+    slice.slice t #s #n #m
   {{{ RET #(slice.slice_f s t n m);
       (* before the sliced part *)
       (slice.slice_f s t (W64 0) n) ↦* (take (uint.nat n) vs) ∗
@@ -905,12 +902,13 @@ Lemma wp_slice_for_range {stk E} sl dq (vs : list V) (body : val) Φ :
                  WP body #i #v @ stk ; E {{ v', ⌜ v' = execute_val #()%V ⌝ ∗ P (word.add i 1) }})
     (λ (_ : w64), sl ↦*{dq} vs -∗ Φ (execute_val #()))
     vs) (W64 0) -∗
-  WP slice.for_range #t #sl body @ stk ; E {{ Φ }}
+  WP slice.for_range t #sl body @ stk ; E {{ Φ }}
 .
 Proof.
   iIntros "Hsl HΦ".
   wp_call.
-  wp_alloc j_ptr as "Hi".
+  wp_apply wp_ref_ty.
+  iIntros (j_ptr) "Hi".
   wp_pures.
   iAssert (
       ∃ (j : u64),
@@ -920,9 +918,11 @@ Proof.
   { iExists (W64 0). iFrame. }
   wp_for "Hinv".
   iDestruct (own_slice_len with "Hsl") as %Hlen.
-  wp_if_destruct.
+  case_bool_decide as Hlt.
   - (* Case: execute loop body *)
-    wp_auto.
+    wp_pures.
+    wp_load.
+    wp_pures.
     pose proof (list_lookup_lt vs (uint.nat j) ltac:(word)) as [w Hlookup].
     iDestruct (own_slice_elem_acc with "[$]") as "[Helem Hown]"; [eassumption|].
     wp_load.
@@ -945,7 +945,7 @@ Qed.
 
 Lemma wp_slice_literal {stk E} (l : list V) :
   {{{ True }}}
-    slice.literal #t #l @ stk ; E
+    slice.literal t #l @ stk ; E
   {{{ sl, RET #sl; sl ↦* l }}}.
 Proof.
   iIntros (Φ) "_ HΦ".
@@ -1077,7 +1077,7 @@ Qed.
 
 Lemma wp_load_slice_elem s (i: w64) (vs: list V) dq v :
   {{{ s ↦*{dq} vs ∗ ⌜vs !! (uint.nat i) = Some v⌝ }}}
-    ![#t] #(slice.elem_ref_f s t i)
+    ![t] #(slice.elem_ref_f s t i)
   {{{ RET #v; s ↦*{dq} vs }}}.
 Proof.
   wp_start_folded as "[Hs %Hlookup]".
@@ -1092,7 +1092,7 @@ Qed.
 
 Lemma wp_store_slice_elem s (i: w64) (vs: list V) (v': V) :
   {{{ s ↦* vs ∗ ⌜uint.Z i < Z.of_nat (length vs)⌝ }}}
-    #(slice.elem_ref_f s t i) <-[#t] #v'
+    store_ty t #(slice.elem_ref_f s t i) #v'
   {{{ RET #(); s ↦* (<[uint.nat i := v']> vs) }}}.
 Proof.
   wp_start_folded as "[Hs %bound]".
@@ -1112,7 +1112,7 @@ Use [take_ge] and [drop_ge] to simplify the resulting list expression.
  *)
 Lemma wp_slice_copy (s: slice.t) (vs: list V) (s2: slice.t) (vs': list V) dq :
   {{{ s ↦* vs ∗ s2 ↦*{dq} vs' }}}
-    slice.copy #t #s #s2
+    slice.copy t #s #s2
   {{{ (n: w64), RET #n; ⌜uint.nat n = Nat.min (length vs) (length vs')⌝ ∗
                           s ↦* (take (length vs) vs' ++ drop (length vs') vs) ∗
                           s2 ↦*{dq} vs' }}}.
@@ -1215,7 +1215,7 @@ Qed.
 
 Lemma wp_slice_append (s: slice.t) (vs: list V) (s2: slice.t) (vs': list V) dq :
   {{{ s ↦* vs ∗ own_slice_cap V s (DfracOwn 1) ∗ s2 ↦*{dq} vs' }}}
-    slice.append #t #s #s2
+    slice.append t #s #s2
   {{{ (s': slice.t), RET #s';
       s' ↦* (vs ++ vs') ∗ own_slice_cap V s' (DfracOwn 1) ∗ s2 ↦*{dq} vs' }}}.
 Proof.
